verif/btrees/verif_putrecord.v
@@ -246,7 +246,7 @@ Proof.
       assert (H98: Zlength le <= Fanout). {apply H2 in SUBNODE.
           apply node_wf_numKeys in SUBNODE. simpl in SUBNODE. rep_omega. }
      forward_if(PROP ( )
-     LOCAL (temp _t'56 (Vint (Int.repr (numKeys currnode)));
+     LOCAL (temp _t'56 (Vint (Int.repr (Zlength (node_le currnode))));
      temp _t'15 (Vint (Int.repr entryidx)); 
      temp _cursor pc; temp _newEntry pe; temp _key (key_repr oldk);
      temp _t'17 (Val.of_bool(key_in_le (entry_key e) le))) (* new local *)
