verif/btrees/verif_splitnode_part2.v
@@ -39,7 +39,7 @@ Lemma splitnode_main_if_then_proof:
    (nval : val) (e : entry val) (pe : val) (gv : globals) (v_allEntries : val)
   (H : node_integrity (btnode val ptr0 le isLeaf First Last nval)),
   let n := btnode val ptr0 le isLeaf First Last nval : node val in
-  forall (H0 : numKeys n = Fanout)
+  forall (H0 : Zlength (node_le n) = Fanout)
   (LEAFENTRY : LeafEntry e = LeafNode (btnode val ptr0 le isLeaf First Last nval))
   (keyrepr : val) (coprepr : val + val)
   (HEVR : entry_val_rep e = (keyrepr, coprepr))
@@ -72,7 +72,7 @@ semax (func_tycontext f_splitnode Vprog Gprog [])
      (Val.of_bool isLeaf,
      (Val.of_bool First,
      (Vint (Int.repr 0),
-     (Vint (Int.repr (numKeys (btnode val ptr0 le isLeaf First Last nval))),
+     (Vint (Int.repr (Zlength (node_le (btnode val ptr0 le isLeaf First Last nval)))),
      (optionally getval nullval ptr0,
       map entry_val_rep le ++ ent_end))))) nval;
    optionally btnode_rep emp ptr0; iter_sepcon entry_rep le;
@@ -209,7 +209,7 @@ Proof.
     assert(0 <= fri < Zlength (map entry_val_rep (sublist 0 fri le) ++ allent_end)).
     { split. omega. rewrite Zlength_app, Zlength_map.
       rewrite Zlength_sublist. rep_omega. rep_omega.
-    change (Zlength le) with (numKeys n). omega. }
+    change (Zlength le) with (Zlength (node_le n)). omega. }
     rewrite upd_Znth_twice by auto. rewrite upd_Znth_same by auto.
     assert(FRILENGTH: Zlength (sublist 0 fri le) = fri).
     { rewrite Zlength_sublist. rep_omega. rep_omega.
