verif/btrees/verif_splitnode_part3.v
@@ -37,7 +37,7 @@ Lemma splitnode_main_ifelse_part2_proof:
     (LEAFENTRY : LeafEntry (keychild val ke ce) =
             LeafNode (btnode val ptr0 le false First Last nval)),
    let n := btnode val ptr0 le false First Last nval : node val in 
-   forall (H0 : numKeys n = Fanout)
+   forall (H0 : Zlength (node_le n) = Fanout)
       (H : node_integrity (btnode val ptr0 le false First Last nval)) 
       (k : key) (fri : Z) 
       (HFRI : findRecordIndex n k = fri)
